Challenge/Modexp/Submission/Proofs/Fast/CiosCachedPrograms.lean
@@ -85,8 +85,7 @@ def l2Program (w : Fin 33) (x tl ts : UInt256) : List Instr :=
     macProductProgram) ++ macFinishProgram tl ts
 
 def entryProgram : List Instr :=
-  [
-   .op .JUMPDEST,
+  [.op .JUMPDEST,
    .push 1 31,
    .op .NOT,
    .push 2 9344,
@@ -95,10 +94,10 @@ def entryProgram : List Instr :=
    .op .EQ,
    .push 1 153,
    .op .MUL,
-   .push 2 4281,
+   .push 2 4280,
    .op .ADD,
    .op (.Dup ⟨0, by decide⟩),
-   .push 3 299,
+   .push 2 291,
    .op .ADD,
    .op (.Swap ⟨3, by decide⟩),
    .push 0 0,
@@ -107,7 +106,7 @@ def entryProgram : List Instr :=
    .push 2 9344,
    .op .MLOAD,
    .op (.Dup ⟨0, by decide⟩),
-   .push 5 64,
+   .push 1 64,
    .op .ADD,
    .op .CALLDATASIZE,
    .push 2 8192,
@@ -182,7 +181,7 @@ def tailProgram : List Instr :=
    .op (.Dup ⟨2, by decide⟩),
    .op (.Dup ⟨1, by decide⟩),
    .op .GT,
-   .push 2 4250,
+   .push 2 4252,
    .op .JUMPI,
    .op .POP,
    .op .POP,
@@ -191,7 +190,7 @@ def tailProgram : List Instr :=
    .op .POP,
    .op .POP,
    .op .POP,
-   .push 2 2139,
+   .push 2 4973,
    .op .JUMP]
 
 def l1DispatchProgram : List Instr :=
